@@ -45,6 +45,7 @@ import MachCSL.WpLock
 import MachCSL.WpSmodeMem2
 import MachCSL.WpSmodeBits
 import MachCSL.Pte
+import MachCSL.KMap
 import MachCSL.PtTree
 import MachCSL.KptInv
 import MachCSL.WpPtWalk
